dimsum_examples/imp_heap_bij_pure.v
@@ -3,6 +3,8 @@ From dimsum.core Require Import link prepost.
 From dimsum.core Require Import axioms.
 From dimsum.examples Require Import imp.
 
+(** * Pure version of [imp_heap_bij] *)
+
 Module pure_bij.
 Implicit Types (p : prov).
 
@@ -14,7 +16,7 @@ Proof. solve_decision. Qed.
 Global Instance heap_bij_elem_inhabited : Inhabited heap_bij_elem := populate (HBOwned Prog).
 
 (* Naming scheme: pi for provenances in the implementation (right side
-of hb_bij), ps for provanences in the spec (left side) *)
+of hb_bij), ps for provanences in the spec (left side of hb_bij) *)
 
 Record heap_bij := HeapBij {
   hb_bij : gmap prov heap_bij_elem;
@@ -47,7 +49,7 @@ Global Program Instance imp_heap_bij_empty : Empty heap_bij :=
   HeapBij ∅ ∅ _ _.
 Solve Obligations with set_solver.
 
-(** hb_shared_i *)
+(** ** hb_shared_i *)
 Definition hb_shared_i (bij : heap_bij) : gset prov :=
   list_to_set (omap (λ x, if x.2 is HBShared p then Some p else None) (map_to_list (hb_bij bij))).
 Global Typeclasses Opaque hb_shared_i.
@@ -62,7 +64,7 @@ Proof.
   - move => [??]. by eexists (_, _).
 Qed.
 
-(** hb_shared *)
+(** ** hb_shared *)
 Definition hb_shared (bij : heap_bij) : gmap prov prov :=
   (omap (λ v, if v is HBShared p then Some p else None) (hb_bij bij)).
 
@@ -78,14 +80,14 @@ Lemma hb_shared_lookup_None bij ps :
   hb_shared bij !! ps = None ↔ ∀ pi, hb_bij bij !! ps = Some (HBShared pi) → False.
 Proof. rewrite hb_shared_lookup. destruct (hb_bij bij !! ps) => //=. case_match; naive_solver. Qed.
 
-(** hb_shared_s *)
+(** ** hb_shared_s *)
 Definition hb_shared_s (bij : heap_bij) : gset prov := dom (hb_shared bij).
 
 Lemma elem_of_hb_shared_s bij ps :
   ps ∈ hb_shared_s bij ↔ ∃ pi, hb_bij bij !! ps = Some (HBShared pi).
 Proof. rewrite /hb_shared_s; unlock. rewrite elem_of_dom /is_Some. f_equiv => ?. apply hb_shared_lookup_Some. Qed.
 
-(** hb_player_s *)
+(** ** hb_player_s *)
 Definition hb_player_s (pl : player) (bij : heap_bij) : gset prov :=
   dom (filter (λ '(k, e), e = HBOwned pl) (hb_bij bij)).
 
@@ -104,7 +106,7 @@ Lemma hb_player_s_empty pl bij :
   hb_player_s pl bij = ∅ ↔ (∀ ps, hb_bij bij !! ps ≠ Some (HBOwned pl)).
 Proof. rewrite set_eq. setoid_rewrite elem_of_hb_player_s. set_solver. Qed.
 
-(** hb_player_i *)
+(** ** hb_player_i *)
 Definition hb_player_i (pl : player) (bij : heap_bij) : gset prov :=
   dom (filter (λ '(k, e), e = pl) (hb_players_i bij)).
 
@@ -123,7 +125,7 @@ Lemma hb_player_i_empty pl bij :
   hb_player_i pl bij = ∅ ↔ (∀ ps, hb_players_i bij !! ps ≠ Some pl).
 Proof. rewrite set_eq. setoid_rewrite elem_of_hb_player_i. set_solver. Qed.
 
-(** hb_provs_i *)
+(** ** hb_provs_i *)
 (* hb_provs_s is directly written as [dom _ (hb_bij bij)] *)
 
 Definition hb_provs_i (bij : heap_bij) : gset prov :=
@@ -133,7 +135,7 @@ Lemma elem_of_hb_provs_i bij pi :
   pi ∈ hb_provs_i bij ↔ (∃ pl, hb_players_i bij !! pi = Some pl) ∨ ∃ ps, hb_bij bij !! ps = Some (HBShared pi).
 Proof. unfold hb_provs_i. rewrite elem_of_union elem_of_dom elem_of_hb_shared_i. naive_solver. Qed.
 
-(** general hb_bij *)
+(** ** general hb_bij *)
 Lemma heap_bij_eq_parts bij1 bij2 :
   bij1 = bij2 ↔
     hb_shared bij1 = hb_shared bij2 ∧
@@ -168,7 +170,7 @@ Global Typeclasses Opaque heap_bij_extend.
 
 Local Ltac bij_solver := unfold heap_bij_extend, subseteq, heap_bij_subseteq in *; set_unfold; naive_solver.
 
-(** heap_bij constructors *)
+(** ** heap_bij constructors *)
 Program Definition heap_bij_add_shared (pi ps : prov) (bij : heap_bij)
         (H : pi ∉ hb_provs_i bij) :=
   HeapBij (<[ps := HBShared pi]> (hb_bij bij)) (hb_players_i bij) _ _.
@@ -206,38 +208,7 @@ Next Obligation.
   rewrite !lookup_delete_Some => ??. destruct!/= => //. by apply: hb_iff.
 Qed.
 
-(* Definition heap_bij_map_player_bij (f : prov → player → player) (bij : heap_bij) : gmap prov heap_bij_elem := *)
-(*   map_imap (λ ps e, Some $ if e is HBOwned p then HBOwned (f ps p) else e) (hb_bij bij). *)
-
-(* Lemma heap_bij_map_player_bij_lookup f bij p2 : *)
-(*   heap_bij_map_player_bij f bij !! p2 = *)
-(*     (λ x, if x is HBOwned p then HBOwned (f p2 p) else x) <$> hb_bij bij !! p2. *)
-(* Proof. rewrite map_lookup_imap. by destruct (hb_bij bij !! p2). Qed. *)
-
-(* Lemma heap_bij_map_player_bij_lookup_shared f bij p2 p1: *)
-(*   heap_bij_map_player_bij f bij !! p2 = Some (HBShared p1) ↔ hb_bij bij !! p2 = Some (HBShared p1). *)
-(* Proof. *)
-(*   rewrite heap_bij_map_player_bij_lookup. rewrite fmap_Some. split; [|naive_solver]. *)
-(*   move => [[?|?][??]]//. naive_solver. *)
-(* Qed. *)
-
-(* Program Definition heap_bij_map_player (f : prov → player → player) (bij : heap_bij) := *)
-(*   HeapBij (heap_bij_map_player_bij f bij) _. *)
-(* Next Obligation. *)
-(*   move => ?????? /heap_bij_map_player_bij_lookup_shared?/heap_bij_map_player_bij_lookup_shared?. apply: hb_iff; naive_solver. *)
-(* Qed. *)
-
-(* Lemma heap_bij_map_player_subseteq_l f bij1 bij2: *)
-(*   heap_bij_map_player f bij1 ⊆ bij2 ↔ bij1 ⊆ bij2. *)
-(* Proof. unfold subseteq, heap_bij_subseteq. by setoid_rewrite heap_bij_map_player_bij_lookup_shared. Qed. *)
-
-(* Lemma heap_bij_map_player_subseteq_r f bij1 bij2: *)
-(*   bij1 ⊆ heap_bij_map_player f bij2 ↔ bij1 ⊆ bij2. *)
-(* Proof. unfold subseteq, heap_bij_subseteq. by setoid_rewrite heap_bij_map_player_bij_lookup_shared. Qed. *)
-
-(* (* Lemma elem_of_hb_player_s_map p x f bij : *) *)
-(* (*   x ∈ hb_player_s p (heap_bij_map_player f bij) ↔ f  *) *)
-
+(** ** Merging two bijections *)
 (* only provenances which are shared in both bijections become shared
 in the merged bijection, otherwise they become private. *)
 Program Definition heap_bij_merge (bija bijb : heap_bij) :=
@@ -415,195 +386,6 @@ Proof.
      split; [|naive_solver congruence]. apply heap_bij_merge_shared. naive_solver.
 Qed.
 
-(*
-(** ** expr_in_bij *)
-Fixpoint expr_in_bij (bij : heap_bij) (e1 e2 : expr) {struct e1} : Prop :=
-  match e1, e2 with
-  | Var v, Var v' => v = v'
-  | Val v, Val v' => val_in_bij bij v v'
-  | BinOp e1 o e2, BinOp e1' o' e2' => o = o' ∧ expr_in_bij bij e1 e1' ∧ expr_in_bij bij e2 e2'
-  | Load e, Load e' => expr_in_bij bij e e'
-  | Store e1 e2, Store e1' e2' => expr_in_bij bij e1 e1' ∧ expr_in_bij bij e2 e2'
-  | Alloc e, Alloc e' => expr_in_bij bij e e'
-  | Free e, Free e' => expr_in_bij bij e e'
-  | If e e1 e2, If e' e1' e2' => expr_in_bij bij e e' ∧ expr_in_bij bij e1 e1' ∧ expr_in_bij bij e2 e2'
-  | LetE v e1 e2, LetE v' e1' e2' => v = v' ∧ expr_in_bij bij e1 e1' ∧ expr_in_bij bij e2 e2'
-  | Call f args, Call f' args' => f = f' ∧ length args = length args' ∧
-                                   Forall id (zip_with (expr_in_bij bij) args args')
-  | UbE, UbE => True
-  | ReturnExt b e, ReturnExt b' e' => b = b' ∧ expr_in_bij bij e e'
-  | Waiting b, Waiting b' => b = b'
-  | _, _ => False
-  end.
-
-Lemma Forall2_bij_val_inv_l bij vl el :
-  Forall2 (expr_in_bij bij) (Val <$> vl) el →
-  ∃ vl', el = Val <$> vl' ∧ Forall2 (val_in_bij bij) vl vl'.
-Proof.
-  elim: vl el; csimpl. { move => ? /Forall2_nil_inv_l->. by eexists []. }
-  move => ?? IH ? /(Forall2_cons_inv_l _ _)[v' [?[?[/IH[?[??]]?]]]]; subst.
-  destruct v' => //. eexists (_::_). split; [done|]. by econs.
-Qed.
-
-Lemma Forall2_bij_val_inv_r bij vl el :
-  Forall2 (expr_in_bij bij) el (Val <$> vl) →
-  ∃ vl', el = Val <$> vl' ∧ Forall2 (val_in_bij bij) vl' vl.
-Proof.
-  elim: vl el; csimpl. { move => ? /Forall2_nil_inv_r->. by eexists []. }
-  move => ?? IH ? /(Forall2_cons_inv_r _ _ _ _) [v' [?[?[/IH[?[??]] ?]]]]; subst.
-  destruct v' => //. eexists (_::_). split; [done|]. by econs.
-Qed.
-
-Lemma expr_in_bij_mono bij bij' e1 e2:
-  expr_in_bij bij e1 e2 →
-  bij ⊆ bij' →
-  expr_in_bij bij' e1 e2.
-Proof.
-  elim: e1 e2 => //=*; repeat case_match => //; try naive_solver (eauto using val_in_bij_mono).
-  destruct!. split!.
-  revert select (Forall id _). generalize dependent args.
-  revert select (Forall _ _). elim. { by case. }
-  move => ????? []//=??? *; decompose_Forall_hyps. econs; naive_solver.
-Qed.
-
-Lemma expr_in_bij_subst bij x v e v' e':
-  expr_in_bij bij e e' →
-  val_in_bij bij v v' →
-  expr_in_bij bij (subst x v e) (subst x v' e').
-Proof.
-  elim: e e' => //= *; repeat (case_match => //); simplify_eq/=; repeat case_bool_decide => //; try naive_solver.
-  destruct_all?. rewrite !fmap_length. split!.
-  revert select (Forall _ _). generalize dependent args.
-  revert select (Forall _ _). elim. { by case. }
-  move => ????? []//=??? /(Forall_cons_1 _ _)[??]. econs; naive_solver.
-Qed.
-
-Lemma expr_in_bij_subst_l bij xs vs e vs' e':
-  expr_in_bij bij e e' →
-  Forall2 (val_in_bij bij) vs vs' →
-  length xs = length vs →
-  expr_in_bij bij (subst_l xs vs e) (subst_l xs vs' e').
-Proof.
-  move => He Hall. elim: Hall xs e e' He. { by case. }
-  move => ?????? IH []//=??????. apply: IH; [|lia]. by apply expr_in_bij_subst.
-Qed.
-
-Lemma expr_in_bij_static bij e:
-  is_static_expr false e →
-  expr_in_bij bij e e.
-Proof.
-  elim: e => //=; try naive_solver. { by case. }
-  move => ?? IH Hb. split!.
-  elim: IH Hb => //=; econs; naive_solver.
-Qed.
-
-(** ** ectx_in_bij *)
-Definition ectx_item_in_bij (bij : heap_bij) (Ki Ki' : expr_ectx) : Prop :=
-  match Ki, Ki' with
-  | BinOpLCtx op e2, BinOpLCtx op' e2' => op = op' ∧ expr_in_bij bij e2 e2'
-  | BinOpRCtx v1 op, BinOpRCtx v1' op' => op = op' ∧ val_in_bij bij v1 v1'
-  | LoadCtx, LoadCtx => True
-  | StoreLCtx e2, StoreLCtx e2' => expr_in_bij bij e2 e2'
-  | StoreRCtx v1, StoreRCtx v1' => val_in_bij bij v1 v1'
-  | AllocCtx, AllocCtx => True
-  | FreeCtx, FreeCtx => True
-  | IfCtx e2 e3, IfCtx e2' e3' => expr_in_bij bij e2 e2' ∧ expr_in_bij bij e3 e3'
-  | LetECtx v e2, LetECtx v' e2' => v = v' ∧ expr_in_bij bij e2 e2'
-  | CallCtx f vl el, CallCtx f' vl' el' => f = f' ∧ Forall2 (val_in_bij bij) vl vl' ∧
-                                            Forall2 (expr_in_bij bij) el el'
-  | ReturnExtCtx b, ReturnExtCtx b' => b = b'
-  | _, _ => False
-  end.
-
-Definition ectx_in_bij (bij : heap_bij) (K1 K2 : list expr_ectx) : Prop :=
-  Forall2 (ectx_item_in_bij bij) K1 K2.
-
-Lemma ectx_item_in_bij_mono bij bij' K1 K2:
-  ectx_item_in_bij bij K1 K2 →
-  bij ⊆ bij' →
-  ectx_item_in_bij bij' K1 K2.
-Proof.
-  destruct K1, K2 => //=; try naive_solver (eauto using expr_in_bij_mono, val_in_bij_mono).
-  move => [?[??]] ?. split_and!; [done|..].
-  all: apply: Forall2_impl; [done|]; eauto using expr_in_bij_mono, val_in_bij_mono.
-Qed.
-
-Lemma ectx_in_bij_mono bij bij' K1 K2:
-  ectx_in_bij bij K1 K2 →
-  bij ⊆ bij' →
-  ectx_in_bij bij' K1 K2.
-Proof. move => ??. apply: Forall2_impl; [done|]. move => *; by apply: ectx_item_in_bij_mono.  Qed.
-
-Lemma ectx_in_bij_cons bij Ki K Ki' K':
-  ectx_in_bij bij (Ki :: K) (Ki' :: K') ↔ ectx_item_in_bij bij Ki Ki' ∧ ectx_in_bij bij K K'.
-Proof. apply Forall2_cons. Qed.
-
-Lemma ectx_in_bij_app bij Ki K Ki' K':
-  ectx_in_bij bij Ki Ki' →
-  ectx_in_bij bij K K' →
-  ectx_in_bij bij (Ki ++ K) (Ki' ++ K').
-Proof. apply Forall2_app. Qed.
-
-Lemma ectx_in_bij_cons_inv_l bij Ki K K':
-  ectx_in_bij bij (Ki::K) K' →
-  ∃ Ki' K'', ectx_item_in_bij bij Ki Ki' ∧ ectx_in_bij bij K K'' ∧ K' = Ki' :: K''.
-Proof. apply Forall2_cons_inv_l. Qed.
-
-Lemma expr_in_bij_fill_item_2 bij K1 K2 e1 e2 :
-  ectx_item_in_bij bij K1 K2 →
-  expr_in_bij bij e1 e2 →
-  expr_in_bij bij (expr_fill_item K1 e1) (expr_fill_item K2 e2).
-Proof.
-  move => ??.
-  destruct K1, K2 => //; simplify_eq/=; destruct_all? => //.
-  rewrite !app_length /=. split_and!; [done|solve_length|].
-  apply Forall_zip_with_2. apply Forall2_app; [by apply Forall2_fmap|by econs].
-Qed.
-
-Lemma expr_in_bij_fill_2 bij K1 K2 e1 e2 :
-  ectx_in_bij bij K1 K2 →
-  expr_in_bij bij e1 e2 →
-  expr_in_bij bij (expr_fill K1 e1) (expr_fill K2 e2).
-Proof.
-  elim: K1 K2 e1 e2. { move => ??? /Forall2_nil_inv_l->. done. }
-  move => Ki1 K1 IH ??? /(Forall2_cons_inv_l _ _)[Ki2 [K2 [?[??]]]] ?; subst => /=.
-  apply: IH; [done|]. by apply expr_in_bij_fill_item_2.
-Qed.
-
-Lemma expr_in_bij_fill_item_l bij Ki e1 e2 :
-  expr_in_bij bij (expr_fill_item Ki e1) e2 →
-  ∃ Ki' e', e2 = expr_fill_item Ki' e' ∧ ectx_item_in_bij bij Ki Ki' ∧ expr_in_bij bij e1 e'.
-Proof.
-  destruct Ki, e2 => //= *; destruct!; try case_match => //; simplify_eq. 10: {
-    revert select (Forall _ _) => /Forall_zip_with_1 Hall.
-    move: (Hall ltac:(done)) => /Forall2_app_inv_l[?[?[Hv[/(Forall2_cons_inv_l _ _)[?[?[?[??]]]]?]]]]. simplify_eq.
-    move: Hv => /Forall2_bij_val_inv_l[?[??]]. simplify_eq.
-    by eexists (CallCtx _ _ _), _.
-  }
-  all: (unshelve eexists _); [econs; shelve| naive_solver].
-Qed.
-
-Lemma expr_in_bij_fill_l bij K e1 e2 :
-  expr_in_bij bij (expr_fill K e1) e2 →
-  ∃ K' e', e2 = expr_fill K' e' ∧ ectx_in_bij bij K K' ∧ expr_in_bij bij e1 e'.
-Proof.
-  elim: K e1 e2 => /=. { move => *. eexists [], _. split!. econs. }
-  move => Ki K IH e1 e2 /IH[K'[?[?[?/expr_in_bij_fill_item_l?]]]].
-  destruct!. eexists (_ :: _), _ => /=. split_and!; [done| |done].
-  by econs.
-Qed.
-
-Lemma eval_binop_bij o v1 v2 v1' v2' v bij:
-  eval_binop o v1 v2 = Some v →
-  val_in_bij bij v1' v1 →
-  val_in_bij bij v2' v2 →
-  ∃ v', eval_binop o v1' v2' = Some v' ∧
-       val_in_bij bij v' v.
-Proof.
-  destruct o, v1, v2, v1', v2' => //= *; destruct!. all: split!.
-  lia.
-Qed.
-*)
 (** *** heap_in_bij *)
 Definition heap_in_bij (bij : heap_bij) (h h' : heap_state) : Prop :=
   ∀ p1 p2 o,
@@ -690,33 +472,6 @@ Proof.
   move => ?; subst => /=. by apply: Hin.
 Qed.
 
-(*
-Lemma heap_in_bij_alloc l1 l2 hi hs n bij H1:
-  heap_in_bij bij hi hs →
-  heap_is_fresh hi l1 →
-  heap_is_fresh hs l2 →
-  (∀ p, hb_bij bij !! l2.1 = Some (HBShared p) → False) →
-  heap_in_bij (heap_bij_add_shared l1.1 l2.1 bij H1) (heap_alloc hi l1 n) (heap_alloc hs l2 n).
-Proof.
-  move => /= Hbij [Hi1 ?] [Hi2 ?] ?  p1 p2 o /= /lookup_insert_Some[[??]|[??]]; simplify_eq.
-  - destruct l1 as [p1 ?], l2 as [p2 ?]; simplify_eq/=.
-    rewrite !lookup_union_l'.
-    2: { apply eq_None_ne_Some => ??. apply Hi2. by apply: (heap_wf _ (_, _)). }
-    2: { apply eq_None_ne_Some => ??. apply Hi1. by apply: (heap_wf _ (_, _)). }
-    split.
-    + rewrite !list_to_map_lookup_is_Some. f_equiv => ?. rewrite !elem_of_list_fmap.
-      f_equiv => ?. naive_solver.
-    + move => ?? /(elem_of_list_to_map_2 _ _ _)/elem_of_list_fmap[?[??]].
-      move => /(elem_of_list_to_map_2 _ _ _)/elem_of_list_fmap[?[??]]. by simplify_eq/=.
-  - have ? : p1 ≠ l1.1. { contradict H1. apply elem_of_hb_shared_i. naive_solver. }
-    have [Hbij1 Hbij2]:= Hbij p1 p2 o ltac:(set_solver).
-    rewrite !lookup_union_r.
-    2, 3: apply not_elem_of_list_to_map_1;
-        move => /elem_of_list_fmap[[[??]?] [?/elem_of_list_fmap[?[??]]]]; simplify_eq/=.
-    split; [done|] => *. apply: val_in_bij_mono; [naive_solver|].
-    move => ??/=?. apply lookup_insert_Some. naive_solver.
-Qed.
-*)
 Lemma heap_in_bij_alloc_r l2 hi hs n bij:
   heap_in_bij bij hi hs →
   (∀ p, hb_bij bij !! l2.1 = Some (HBShared p) → False) →
@@ -751,7 +506,8 @@ Proof.
   naive_solver.
 Qed.
 
-(** *** heap_preserved *)
+(** ** heap_preserved *)
+(* TODO: This is shadowing the definition from imp.v. *)
 Definition heap_preserved (ps : gset prov) (h h' : heap_state) :=
   ∀ p o, p ∈ ps → h.(h_heap) !! (p, o) = h'.(h_heap) !! (p, o).
 
@@ -1383,453 +1139,3 @@ Proof.
 Qed.
 
 End pure_bij.
-
-
-(*
-
-Local Ltac split_solve :=
-  match goal with
-  (* | |- heap_in_bij ?p _ _ => is_evar p; eassumption *)
-  | |- heap_in_bij _ _ _ => apply: heap_in_bij_mono; [eassumption|..]
-  | |- event_set_vals_heap _ _ _ = event_set_vals_heap _ _ _ => reflexivity
-  | |- heap_bij_extend ?p ?a ?b =>
-      assert_fails (has_evar p); assert_fails (has_evar a); assert_fails (has_evar b); by etrans
-  (* | |- ?a ⊆ ?b => *)
-      (* assert_fails (has_evar a); assert_fails (has_evar b); etrans; [eassumption|] *)
-  (* | |- ?a ⊆ ?b => *)
-      (* assert_fails (has_evar a); assert_fails (has_evar b); etrans; [|eassumption] *)
-  | |- _ ⊆ heap_bij_map_player _ _ => apply heap_bij_map_player_subseteq_r
-  | |- heap_bij_map_player _ _ ⊆ _ => apply heap_bij_map_player_subseteq_l
-  | |- heap_preserved ?p ?a ?b =>
-      assert_fails (has_evar p); assert_fails (has_evar a); assert_fails (has_evar b); etrans; [eassumption|]
-  end.
-Local Ltac split_tac ::=
-  repeat (original_split_tac; try split_solve).
-
-Lemma imp_heap_bij_combine fns1 fns2 m1 m2 σ1 σ2 `{!VisNoAll m1} `{!VisNoAll m2}:
-  trefines (MS (imp_prod fns1 fns2 (imp_heap_bij m1) (imp_heap_bij m2))
-               (MLFNone, [], initial_imp_heap_bij_state m1 σ1,
-                 initial_imp_heap_bij_state m2 σ2))
-           (MS (imp_heap_bij (imp_prod fns1 fns2 m1 m2))
-               (initial_imp_heap_bij_state (imp_prod _ _ _ _)
-                  (MLFNone, [], σ1, σ2) )
-).
-Proof.
-  unshelve apply: mod_prepost_link. { exact
-      (λ ips '(ImpHeapBij bij1 hi1) '(ImpHeapBij bij2 hi2) '(ImpHeapBij bij hi) _ _ ics1 ics2,
-        ∃ bijm,
-          ics1 = ics2 ∧
-          bij1 ⊆ bijm ∧
-          bij2 ⊆ bijm ∧
-          bij ⊆ bijm ∧
-       ((ips = SPNone ∧ bijm = bij ∧
-          hb_player Prog bij = hb_player Prog bij1 ∪ hb_player Prog bij2 ∧
-          hb_player Prog bij1 ## hb_player Prog bij2 ∧
-          heap_preserved (hb_player Prog bij1) hi1 hi ∧
-          heap_preserved (hb_player Prog bij2) hi2 hi) ∨
-        ((ips = SPLeft ∧ bijm = bij1 ∧
-          hb_player Env bij1 = hb_player Env bij ∪ hb_player Prog bij2 ∧
-          hb_player Prog bij2 ## hb_player Env bij ∧
-          heap_preserved (hb_player Env bij) hi hi1 ∧
-          heap_preserved (hb_player Prog bij2) hi2 hi1) ∨
-         (ips = SPRight ∧ bijm = bij2 ∧
-          hb_player Env bij2 = hb_player Env bij ∪ hb_player Prog bij1 ∧
-          hb_player Prog bij1 ## hb_player Env bij ∧
-          heap_preserved (hb_player Env bij) hi hi2 ∧
-          heap_preserved (hb_player Prog bij1) hi1 hi2)))). }
-  { move => ?? [] /=*; naive_solver. }
-  { by rewrite left_id. } { by apply satisfiable_pure_1. }
-  { split!.  all: rewrite /hb_player; unlock; set_solver. }
-  all: move => [bij1 hi1] [bij2 hi2] [bij hi] ? ? ics1 ics2.
-  - move => e ics' e' /= *. unfold heap_bij_extend in *. destruct!/=.
-    eexists (heap_bij_map_player (λ p2 p, if decide (p2 ∈ hb_player Prog bij2) then Env else p) bij).
-    split!.
-    { set_unfold.
-    1: {
-1: econstructor. all: shelve_unifiable. all: split!. all: split!.
-    1: { apply: heap_preserved_mono; [done|]. set_unfold; naive_solver. }
-    1: by iIntros "$".
-    1: by destruct e.
-    1: { apply: disjoint_mono; [apply hb_disj_priv| |done]. set_unfold; naive_solver. }
-    1: { apply: heap_preserved_mono; [done|]. set_unfold; naive_solver. }
-  - move => e ics' e' /= *. unfold heap_bij_extend in *; destruct!/=.
-    unshelve split!. 1: econstructor. all: shelve_unifiable. all: split!. all: split!.
-    1: { apply: heap_preserved_mono; [done|]. set_unfold; naive_solver. }
-    1: by iIntros "$".
-    1: by destruct e.
-    1: { apply: disjoint_mono; [apply hb_disj_priv| |done]. set_unfold; naive_solver. }
-    1: { apply: heap_preserved_mono; [done|]. set_unfold; naive_solver. }
-  - move => [? e] /= *. unfold heap_bij_extend in *; destruct!/=.
-    unshelve split!. 1: econstructor. all: shelve_unifiable.
-    all: split!; rewrite ?heap_of_event_event_set_vals_heap; split!. all: split!.
-    1: { rewrite vals_of_event_event_set_vals_heap //. by apply: Forall2_length. }
-    1: { apply: heap_preserved_mono; [done|]. set_unfold; naive_solver. }
-    1: { iIntros "[? $]". iStopProof. etrans; [done|]. by iIntros ">[_ $]". }
-    1: { apply: disjoint_mono; [apply hb_disj_priv|done|]. set_unfold; naive_solver. }
-    1: { apply: heap_preserved_mono; [done|]. set_unfold; naive_solver. }
-    1: by destruct e.
-    1: by destruct e.
-  - move => [? e] /= *. unfold heap_bij_extend in *; destruct!/=.
-    unshelve split!. 1: econstructor. all: shelve_unifiable.
-    all: split!; rewrite ?heap_of_event_event_set_vals_heap; split!. all: split!.
-    1: by destruct e.
-    1: { apply: heap_preserved_mono; [done|]. set_unfold; naive_solver. }
-    1: { etrans; [done|]. iIntros ">[? $]". iStopProof. etrans; [done|]. by iIntros ">[_ $]". }
-    1: { apply: disjoint_mono; [apply hb_disj_priv|done|]. set_unfold; naive_solver. }
-    1: { apply: heap_preserved_mono; [done|]. set_unfold; naive_solver. }
-  - move => [? e] /= *. unfold heap_bij_extend in *; destruct!/=.
-    unshelve split!. 1: econstructor. all: shelve_unifiable.
-    all: split!; rewrite ?heap_of_event_event_set_vals_heap; split!. all: split!.
-    1: { rewrite vals_of_event_event_set_vals_heap //. by apply: Forall2_length. }
-    1: { apply: heap_preserved_mono; [done|]. set_unfold; naive_solver. }
-    1: { iIntros "[$ ?]". iStopProof. etrans; [done|]. by iIntros ">[_ $]". }
-    1: { apply: disjoint_mono; [apply hb_disj_priv|done|]. set_unfold; naive_solver. }
-    1: { apply: heap_preserved_mono; [done|]. set_unfold; naive_solver. }
-    1: by destruct e.
-    1: by destruct e.
-  - move => [? e] /= *. unfold heap_bij_extend in *; destruct!/=.
-    unshelve split!. 1: econstructor. all: shelve_unifiable.
-    all: split!; rewrite ?heap_of_event_event_set_vals_heap; split!. all: split!.
-    1: by destruct e.
-    1: { apply: heap_preserved_mono; [done|]. set_unfold; naive_solver. }
-    1: { etrans; [done|]. iIntros ">[$ ?]". iStopProof. etrans; [done|]. by iIntros ">[_ $]". }
-    1: { symmetry. apply: disjoint_mono; [apply hb_disj_priv|done|]. set_unfold; naive_solver. }
-    1: { apply: heap_preserved_mono; [done|]. set_unfold; naive_solver. }
-    Unshelve.
-    (* We need to use abstract here as otherwise Qed does not terminate. *)
-    all: try abstract (by apply hb_iff).
-    all: abstract (
-      try (apply disjoint_union_l; split);
-      try (apply disjoint_union_r; split);
-      try (by apply hb_disj_env);
-      try (by apply hb_disj_prog);
-      try done;
-      try (apply: disjoint_mono; [apply hb_disj_prog| |done]; apply: subseteq_mono_eq_r; [|eassumption]);
-      try (apply: disjoint_mono; [apply hb_disj_priv| |done]; apply: subseteq_mono_eq_r; [|eassumption]);
-      try (apply: disjoint_mono; [apply hb_disj_env| |done]; apply: subseteq_mono_eq_r; [|eassumption]);
-      try (apply: disjoint_mono; [apply hb_disj_priv|done|]; apply: subseteq_mono_eq_r; [|eassumption]);
-      try (symmetry; apply: disjoint_mono; [apply hb_disj_priv|done|]; apply: subseteq_mono_eq_r; [|eassumption]);
-      set_unfold; naive_solver).
-Qed.
-
-
-Local Ltac split_solve ::=
-  match goal with
-  | |- expr_fill (?K' ++ ?K) _ = expr_fill ?K _ =>
-      assert_fails (has_evar K'); assert_fails (has_evar K); apply expr_fill_app
-  | |- expr_fill ?K _ = expr_fill ?K _ =>
-      assert_fails (has_evar K); reflexivity
-  | |- Is_true (is_static_expr _ (expr_fill _ _)) => apply is_static_expr_expr_fill
-  | |- expr_in_bij ?b (expr_fill _ _) (expr_fill _ _) =>
-      assert_fails (has_evar b); apply expr_in_bij_fill_2
-  | |- ectx_in_bij ?b (_ ++ _) (_ ++ _) => assert_fails (has_evar b); by apply ectx_in_bij_app
-  end.
-Local Ltac split_tac ::=
-  repeat (original_split_tac; try split_solve).
-
-Local Ltac bij_solver := unfold heap_bij_extend in *; set_unfold; naive_solver.
-
-Lemma imp_heap_bij_imp_refl fns:
-  trefines (MS imp_module (initial_imp_state fns))
-           (MS (imp_heap_bij imp_module)
-               (initial_imp_heap_bij_state imp_module (initial_imp_state fns))).
-Proof.
-  epose (R := λ (b : bool) '(ImpHeapBij bij1 h1, _) '(ImpHeapBij bij2 h2, _),
-          (hb_prog bij1 = ∅ → hb_prog bij2 = ∅) ∧ hb_bij bij1 ⊆ hb_bij bij2).
-  apply: (imp_prepost_proof R); unfold R in *.
-  { constructor. { move => [[??]?]. naive_solver. }
-    { move => [[??]?] [[??]?] [[??]?] [??] [??]. split. naive_solver. by etrans. } }
-  { move => [??] ? [??] ?. naive_solver. }
-  move => n K1 K2 f fn1 vs1 h1 [bij0 ?] ??? /= bij1 *.
-  split!. move => ?. split; [solve_length|].
-  move => Hcall Hret.
-  unshelve apply: tsim_remember. { simpl. exact (λ _ '(Imp ei hi fnsi) '(ips, Imp es hs fnss, (pp, ImpHeapBij bij he, P)),
-    (* bij' : current bijection, bij : bijection when last communicated with the environment,
-     bij1: bijection at the start of the function (necessary to reestablish R) *)
-    ∃ bij' ei' es',
-    fnsi = fns ∧ fnss = fns ∧
-    hb_env bij = hb_env bij' ∧
-    hb_prog bij = ∅ ∧ hb_prog bij' = ∅ ∧
-    hb_bij bij ⊆ hb_bij bij' ∧
-    hb_bij bij1 ⊆ hb_bij bij ∧
-    heap_preserved (hb_env bij') he hs ∧
-    ei = expr_fill K1 ei' ∧
-    es = expr_fill K2 es' ∧
-    expr_in_bij (hb_bij bij') ei' es' ∧
-    heap_in_bij (hb_bij bij') hi hs ∧
-    set_map fst (hb_bij bij') ⊆ h_provs hi ∧
-    pp = PPInside ∧
-    is_static_expr true ei' ∧
-    ips = SMProg
- ). }
-  { eexists _. split!. done. all: split!.
-    { unfold heap_bij_extend in *. clear Hcall Hret. bij_solver. }
-    { unfold heap_bij_extend in *. clear Hcall Hret. bij_solver. }
-    { apply expr_in_bij_subst_l; [|done|solve_length]. apply expr_in_bij_static. apply fd_static. }
-    { apply is_static_expr_subst_l; [|solve_length]. apply is_static_expr_mono. apply fd_static. }   }
-  { naive_solver. }
-  move => /= n' ? Hloop [ei hi fnsi] [[ips [es hs fnss]] [[pp [bij he]] ?]] ?.
-  destruct!.
-  destruct (to_val ei') eqn:?.
-  - destruct ei' => //; simplify_eq/=. destruct es' => //; simplify_eq/=.
-    apply Hret; [done|]. clear Hloop Hret Hcall. split!.
-    { unfold heap_bij_extend. split!; [done..|]. bij_solver. }
-    all: split!. by econs. { instantiate (1:=True%I). iIntros "? !>". done. }
-    { done. }
-    { etrans; [|done]. etrans; [|done]. bij_solver. }
-  - (* TODO: remove this use of EM *)
-    have [?|?]:= EM (∃ K f vs, fns !! f = None ∧ ei' = expr_fill K (Call f (Val <$> vs))).
-    + destruct!/=.
-      revert select (expr_in_bij _ (expr_fill _ _) _) => /expr_in_bij_fill_l[?[?[?[??]]]].
-      destruct!/=.
-      revert select (Is_true (is_static_expr _ _)) => /is_static_expr_expr_fill/=[??]//.
-      case_match => //; destruct!/=.
-      revert select (Forall id _) => /Forall_zip_with_1 Hall.
-      move: (Hall ltac:(done)) => /Forall2_bij_val_inv_l[?[??]]; simplify_eq.
-      apply: Hcall; [done..| | |].
-      1,2: by apply Forall2_fmap_l, Forall_Forall2_diag, Forall_true.
-      clear Hret. split!.
-      { unfold heap_bij_extend. split!; [done..|]. bij_solver. }
-      all: split!.
-      { instantiate (1:=True%I). iIntros "? !>". done. }
-      { etrans; [|done]. etrans; [|done]. bij_solver. }
-      move => ?? [??] *. decompose_Forall_hyps. split!.
-      apply Hloop; [done|]. split!. 1: done. all: split!.
-      1: bij_solver.
-      1: bij_solver.
-      { etrans; [done|]. etrans; [done|]. bij_solver. }
-      { apply: ectx_in_bij_mono; [done|]. bij_solver. }
-    + tstep_both.
-      apply steps_impl_step_end => ?? /= Hprim.
-      move: Hprim => /prim_step_inv[//|??].
-      destruct!.
-      revert select (expr_in_bij _ (expr_fill _ _) _) => /expr_in_bij_fill_l[?[?[?[??]]]].
-      destruct!.
-      revert select (Is_true (is_static_expr _ _)) => /is_static_expr_expr_fill/=[??]//.
-      invert_all' @head_step; destruct!/=.
-      all: repeat (case_match; destruct_all? => //); simplify_eq.
-      * tstep_s => ? /eval_binop_bij Hbin. have [?[??]]:= Hbin _ _ _ ltac:(done) ltac:(done).
-        tend. split!. apply: Hloop; [done|]. split!. 1: done. 1: done. all: split!.
-      * tstep_s => *; simplify_eq/=. destruct v1 => //; simplify_eq/=; destruct!/=. tend.
-        have [//|?[??]]:= heap_in_bij_lookup _ _ _ _ _ _ ltac:(done) ltac:(done) ltac:(done).
-        split!. 1: done.
-        apply: Hloop; [done|]. split!. 1: done. 1: done. all: split!.
-      * tstep_s => *; simplify_eq/=. destruct v1 => //; simplify_eq/=; destruct!/=. tend.
-        split!. 1: by apply: heap_in_bij_alive.
-        apply: Hloop; [done|]. split!. 1: done. 1: done. all: split!.
-        1: by apply: heap_preserved_bij_env.
-        1: by apply heap_in_bij_update.
-      * tstep_s => *; simplify_eq/=.
-        set (l' := (heap_fresh (hb_provs_right bij') hs)).
-        eexists l'. split; [apply heap_fresh_is_fresh|] => *; simplify_eq/=. tend.
-        destruct v => //; simplify_eq/=; destruct!/=.
-        split!.
-        apply Hloop; [done|].
-        unshelve eexists (heap_bij_add_loc l.1 l'.1 bij' _ _).
-        { abstract (apply: not_elem_of_weaken; [|done]; unfold heap_is_fresh in *; naive_solver). }
-        { apply: heap_fresh_not_in. }
-        split!.
-        1: bij_solver.
-        1: { apply heap_preserved_alloc_r; [|done] => ?.
-             apply: (heap_fresh_not_in (hb_provs_right bij') hs). bij_solver. }
-        1: { apply: ectx_in_bij_mono; [done|bij_solver]. }
-        1: bij_solver.
-        1: unfold heap_is_fresh in *; naive_solver.
-        1: { apply: (heap_in_bij_alloc l l').
-             { abstract (apply: not_elem_of_weaken; [|done]; unfold heap_is_fresh in *; naive_solver). }
-             { apply: heap_fresh_not_in. }
-          done. done. apply heap_fresh_is_fresh. }
-        1: bij_solver.
-      * tstep_s => *; simplify_eq/=. tend.
-        destruct v => //; simplify_eq/=; destruct!/=.
-        split!. 1: by apply: heap_in_bij_alive. apply: Hloop; [done|]. split!. 1: done. 1: done. all: split!.
-        1: by apply: heap_preserved_bij_env_free.
-        1: by apply heap_in_bij_free.
-      * tstep_s => *; simplify_eq/=. destruct v => //; simplify_eq/=. tend.
-        split!. apply: Hloop; [done|]. split!. 1: done. 1: done. all: split!. all: by case_match.
-      * tstep_s. tend. split!. apply: Hloop; [done|]. split!. 1: done. all: split!.
-        1: by apply expr_in_bij_subst.
-        1: by apply is_static_expr_subst.
-      * by tstep_s.
-      * revert select (Forall id _) => /Forall_zip_with_1 Hall.
-        move: (Hall ltac:(done)) => /Forall2_bij_val_inv_l[?[??]]; simplify_eq.
-        tstep_s. left. split! => ?. tend. split!; [solve_length|].
-        apply Hloop; [done|]. split!. 1: done. all: split!.
-        1: { apply expr_in_bij_subst_l; [|done|solve_length]. apply expr_in_bij_static. apply fd_static. }
-        apply is_static_expr_subst_l; [|solve_length]. apply is_static_expr_mono. apply fd_static.
-      * naive_solver.
-Qed.
-
-Lemma imp_heap_bij_imp_closed m σ:
-  trefines (MS (imp_closed (imp_heap_bij m)) (SMFilter, initial_imp_heap_bij_state m σ, ICStart))
-           (MS (imp_closed m) (SMFilter, σ, ICStart)).
-Proof.
-  apply tsim_implies_trefines => /= n.
-  unshelve apply: tsim_remember. { simpl. exact (λ _
-          '(σm1, (σf, σ1, (pp, ImpHeapBij bij hi, _)), σc1)
-          '(σm2, σ2, σc2),
-           σ1 = σ2 ∧ σc1 = σc2 ∧
-             ((σc1 = ICStart ∧ σf = SMFilter ∧ pp = PPOutside ∧ σm1 = σm2 ∧ σm2 = SMFilter ∧ bij = ∅) ∨
-              ( ((∃ e, σf = SMProgRecv e ∧ σm2 = SMProgRecv e) ∨ (σf = SMProg ∧ σm2 = SMProg)
-                 ) ∧ σm1 = SMProg ∧ σc1 = ICRunning ∧ pp = PPInside))
-                             ). }
-  { split!. } { done. }
-  move => {}n _ /= Hloop [[σm1 [[σf σ1] [[pp [bij hi]] ?]]] σc1] [[σm2 σ2] σc2] ?.
-  destruct!/=.
-  - tstep_i. apply steps_impl_step_end => ???. invert_all' @m_step; simplify_eq/=. split!.
-    tstep_s. eexists (Some (inr _)). split!. apply: steps_spec_step_end; [econs|] => ??. simplify_eq/=.
-    tstep_i. apply steps_impl_step_end => ???. invert_all @m_step. split!.
-    tstep_s. eexists (Some (inl _)). split!. apply: steps_spec_step_end; [econs|] => ??. simplify_eq/=.
-    tstep_i => ??; simplify_eq/=.
-    tstep_i. eexists ∅, (ValNum <$> vs), ∅. split!.
-    1: { apply Forall2_fmap. apply Forall_Forall2_diag. by apply Forall_true. }
-    apply: Hloop; [done|]. split!.
-  - tstep_both. apply steps_impl_step_end => κ ??. case_match => *; simplify_eq.
-    + tstep_s.  eexists (Some _). split; [done|]. apply: steps_spec_step_end; [done|] => ??. tend. split!; [done|].
-      apply: Hloop; [done|]. split!.
-    + tstep_s. eexists None. apply: steps_spec_step_end; [done|] => ??. tend. split!; [done|].
-      apply: Hloop; [done|]. split!.
-  - tstep_both. apply steps_impl_step_end => κ ??. tstep_s. eexists _. apply: steps_spec_step_end; [done|] => ??.
-    case_match; tend; (split!; [done|]). 2: { apply: Hloop; [done|]. split!. }
-    tstep_i => ? vs *. tstep_both => *.
-    apply steps_impl_step_end => ???. invert_all @m_step => ?; simplify_eq.
-    + destruct i as [? [? vs' |]]; simplify_eq/=.
-      tstep_s. eexists (Some _). split!.
-      apply: steps_spec_step_end; [econs|]=> /=??. destruct!/=. tend.
-      split!.
-      tstep_both. apply steps_impl_step_end => ???. invert_all @m_step.
-      tstep_s. eexists (None). apply: steps_spec_step_end; [econs|]=> /=??. destruct!/=. tend.
-      have ?: vs0 = ValNum <$> vs'0. {
-        revert select (m_step _ _ _ _) => _.
-        revert select (Forall2 _ _ _). elim: vs'0 vs0; csimpl => *; decompose_Forall_hyps => //.
-        match goal with |- ?x :: _ = _ => destruct x; simplify_eq/= => // end. naive_solver.
-      } subst.
-      split!; [done|].
-      tstep_i. apply steps_impl_step_end => ???. invert_all @m_step. split!.
-      tstep_s. eexists (Some (inr _)). split!. apply: steps_spec_step_end; [econs|] => /=? ->.
-      tstep_i. apply steps_impl_step_end => ???. invert_all @m_step. split!.
-      tstep_s. eexists (Some (inl _)). split!. apply: steps_spec_step_end; [econs|] => /=? ->.
-      tstep_i => ? <-.
-      tstep_i. eexists _, [ValNum _]. split!. 1: done. 1: done. 1: econs; [done|econs]. 1: done. 1: done.
-      apply: Hloop; [done|]. split!.
-    + destruct i as [? []]; simplify_eq/=.
-      tstep_s. eexists (Some _). split!.
-      apply: steps_spec_step_end; [econs|]=> /=??. destruct!/=.
-      tstep_s. eexists None. apply: steps_spec_step_end; [econs|]=> /=??. destruct!/=.
-      destruct vs as [|v ?]; decompose_Forall_hyps. destruct v => //; simplify_eq/=.
-      tend. split!.
-      tstep_i. apply: steps_impl_step_end => ???. invert_all @m_step. split!.
-      tstep_i. apply: steps_impl_step_end => ???. invert_all @m_step. split!.
-      tstep_s. eexists (Some (inr _)). split!.
-      apply: steps_spec_step_end; [econs|]=> /=? ->.
-      tstep_i. apply: steps_impl_step_end => ???. invert_all @m_step.
-Qed.
-
-Lemma imp_heap_bij_trefines_implies_ctx_refines fnsi fnss :
-  dom (gset _) fnsi = dom (gset _) fnss →
-  trefines (MS imp_module (initial_imp_state fnsi))
-           (MS (imp_heap_bij imp_module) (initial_imp_heap_bij_state imp_module (initial_imp_state fnss))) →
-  imp_ctx_refines fnsi fnss.
-Proof.
-  move => Hdom Href C. rewrite /imp_link map_difference_union_r (map_difference_union_r fnss).
-  etrans; [|apply imp_heap_bij_imp_closed].
-  apply mod_seq_map_trefines. { apply _. } { apply _. }
-  etrans. { apply imp_link_refines_prod. apply map_disjoint_difference_r'. }
-  etrans. { apply: imp_prod_trefines. 1: done. 1: apply imp_heap_bij_imp_refl. }
-  etrans. { apply imp_heap_bij_combine; apply _. }
-  apply: mod_prepost_trefines.
-  etrans. 2: { apply imp_prod_refines_link. apply map_disjoint_difference_r'. }
-  rewrite !dom_difference_L Hdom.
-  erewrite map_difference_eq_dom_L => //.
-  apply _.
-Qed.
-
-Module imp_heap_bij_example.
-
-Local Open Scope Z_scope.
-
-Definition bij_alloc : fndef := {|
-  fd_args := [];
-  fd_body := (LetE "tmp" (Alloc (Val 1))
-             (LetE "_" (Store (Var "tmp") (Val 1))
-             (LetE "_" (Call "ext" [])
-             (LetE "res" (Load (Var "tmp"))
-             (LetE "_" (Free (Var "tmp"))
-             (Var "res"))))));
-  fd_static := I;
-|}.
-
-Definition bij_alloc_opt : fndef := {|
-  fd_args := [];
-  fd_body := (LetE "_" (Call "ext" [])
-             (Val 1));
-  fd_static := I;
-|}.
-
-Lemma bij_alloc_opt_refines :
-  trefines (MS imp_module (initial_imp_state (<["f" := bij_alloc_opt]> ∅)))
-           (MS (imp_heap_bij imp_module) (initial_imp_heap_bij_state imp_module
-                                            (initial_imp_state (<["f" := bij_alloc]> ∅)))).
-Proof.
-  epose (R := λ (b : bool) '(ImpHeapBij bij1 h1, _) '(ImpHeapBij bij2 h2, _),
-          hb_prog bij1 ⊆ hb_prog bij2 ∧ heap_preserved (hb_prog bij1) h1 h2).
-  apply: (imp_prepost_proof R); unfold R in *.
-  { constructor. { move => [[??]?]. naive_solver. }
-    { move => [[??]?] [[??]?] [[??]?] [??] [??]. split; [by etrans|]. etrans; [done|].
-      by apply: heap_preserved_mono. } }
-  { move => [??] ? [??] ?. naive_solver. }
-  move => n K1 K2 f fn1 vs1 h0 [bij0 ?] ? ?.
-  rewrite !lookup_insert_Some => ?; destruct_all?; simplify_map_eq/=.
-  move => bij1 ? h1 *. split!. move => ?. split!; [solve_length|].
-  move => Hcall Hret.
-  pose (l := (heap_fresh (hb_provs_right bij1) h1)).
-  have Hf := heap_fresh_not_in (hb_provs_right bij1) h1.
-  tstep_s. eexists l. split!. { apply heap_fresh_is_fresh. }
-  move => *; simplify_eq.
-  tstep_s. tstep_s. move => ? [<-] ?.
-  tstep_s.
-  apply: (Hcall _ _ ([LetECtx _ _]) ([LetECtx _ _])); [done|..].
-  1, 2: by simplify_map_eq. 1,2: by econs.
-  unshelve eexists (heap_bij_add_prog l.1 bij1 _), []. { apply Hf. }
-  split!.
-  { apply heap_in_bij_update_r; [|set_solver]. apply heap_in_bij_alloc_r; [done|set_solver]. }
-  { apply heap_preserved_update_r; [|set_solver]. apply heap_preserved_alloc_r; [set_solver|done]. }
-  { instantiate (1:=True%I). iIntros "? !>". done. }
-  { bij_solver. }
-  { etrans; [apply: heap_preserved_mono; [done|bij_solver]|].
-    apply heap_preserved_update_r; [|bij_solver].
-    apply heap_preserved_alloc_r; [bij_solver|done]. }
-  move => ? h2 [bij2 h3] ? [??] bij4 ? h4 *. decompose_Forall_hyps.
-  split!.
-  tstep_i.
-  tstep_s.
-  tstep_s.
-  move => ?? [<-] /heap_preserved_lookup_r Hlookup.
-  efeed pose proof Hlookup as Hlookup'.
-  { etrans. 2: apply: heap_preserved_mono; [done|]. 1: done. bij_solver. }
-  { bij_solver. } simplify_map_eq/=.
-  tstep_s.
-  tstep_s => *. simplify_eq.
-  tstep_s.
-  apply: Hret; [done|].
-  eexists _, [ValNum 1]. split!. done. all: split!. 1: by econs.
-  { apply heap_in_bij_free_r; [done|]. have ? := hb_disj_prog bij4. bij_solver. }
-  { apply: heap_preserved_free_r; [|done]. have ? := hb_disj_priv bij4. bij_solver. }
-  { instantiate (1:=True%I). iIntros "? !>". done. }
-  1: bij_solver.
-  { apply: heap_preserved_free_r. { have ? := hb_disj_priv bij4. bij_solver. }
-    apply: heap_preserved_mono. 1: etrans; [done|]. 2: bij_solver.
-    etrans. 2: apply: heap_preserved_mono; [done|bij_solver].
-    etrans. 2: apply: heap_preserved_mono; [done|bij_solver].
-    apply heap_preserved_update_r; [|bij_solver].
-    apply heap_preserved_alloc_r; [bij_solver|done]. }
-Qed.
-
-Lemma bij_alloc_ctx_refines :
-  imp_ctx_refines (<["f" := bij_alloc_opt]> ∅) (<["f" := bij_alloc]> ∅).
-Proof.
-  apply: imp_heap_bij_trefines_implies_ctx_refines. { set_solver. }
-  apply bij_alloc_opt_refines.
-Qed.
-End imp_heap_bij_example.
-*)
